Semantic/Fsub/Denotation.lean
@@ -1,1 +1,3 @@
 import Semantic.Fsub.Denotation.Core
+import Semantic.Fsub.Denotation.Rebind
+import Semantic.Fsub.Denotation.Retype
